Cfg has procedures, proofs are still not complete.
There's a case I don't know how to prove in the function call and the
Block case I haven't started writing yet.
The stack frame now saves the location to which the return value of a
function is to be saved.

src/SmallStep.thy
@@ -93,17 +93,17 @@ definition en_callfun :: "fname \<Rightarrow> exp list \<Rightarrow> enabled" wh
 
 (* Takes the actual values list, the parameter names list and returns the valuation new stack_frame
    if it returns none it's because the lists had different length \<Rightarrow> error *)
-fun create_stack_frame :: "vname list \<Rightarrow> val list \<Rightarrow> stack_frame option" where
-  "create_stack_frame [] [] = Some (\<lambda>name. None)"
-| "create_stack_frame (x#xs) [] =  do {
-    sf \<leftarrow> (create_stack_frame xs []);
+fun create_locals_stack_frame :: "vname list \<Rightarrow> val list \<Rightarrow> valuation option" where
+  "create_locals_stack_frame [] [] = Some (\<lambda>name. None)"
+| "create_locals_stack_frame (x#xs) [] =  do {
+    sf \<leftarrow> (create_locals_stack_frame xs []);
     Some (sf (x \<mapsto> None))
   }"
-| "create_stack_frame (x#xs) (y#ys) = do {
-    sf \<leftarrow> (create_stack_frame xs ys);
+| "create_locals_stack_frame (x#xs) (y#ys) = do {
+    sf \<leftarrow> (create_locals_stack_frame xs ys);
     Some (sf (x \<mapsto> Some y))
   }"
-| "create_stack_frame _ _ = None"
+| "create_locals_stack_frame _ _ = None"
   
 fun real_values :: "exp list \<Rightarrow> state \<Rightarrow> (val list \<times> state) option" where
   "real_values [] s = Some ([], s)"
@@ -125,11 +125,11 @@ value "real_values [(Const 1), (Plus (Const 1) (Const 2))] initial_state"
 (* The lhs is evaluated before *)
 definition tr_callfunl :: "lexp \<Rightarrow> fname \<Rightarrow> exp list \<Rightarrow> transformer" where
   "tr_callfunl x f call_params s \<equiv> do {
-    (_, (\<sigma>, \<gamma>, \<mu>)) \<leftarrow> eval_l x s;
+    (addr, (\<sigma>, \<gamma>, \<mu>)) \<leftarrow> eval_l x s;
     (params, locals, _) \<leftarrow> proc_table f;
     (values, (\<sigma>, \<gamma>, \<mu>)) \<leftarrow> real_values call_params (\<sigma>, \<gamma>, \<mu>);
-    sf \<leftarrow> create_stack_frame (params@locals) values;
-    Some (sf#\<sigma>, \<gamma>, \<mu>)
+    sf \<leftarrow> create_locals_stack_frame (params@locals) values;
+    Some ((sf, Ar addr)#\<sigma>, \<gamma>, \<mu>)
   }"
 
 definition tr_callfun :: "vname \<Rightarrow> fname \<Rightarrow> exp list \<Rightarrow> transformer" where
@@ -137,26 +137,25 @@ definition tr_callfun :: "vname \<Rightarrow> fname \<Rightarrow> exp list \<Rig
     let (\<sigma>, \<gamma>, \<mu>) = s;
     (params, locals, _) \<leftarrow> proc_table f;
     (values, (\<sigma>, \<gamma>, \<mu>)) \<leftarrow> real_values call_params (\<sigma>, \<gamma>, \<mu>);
-    sf \<leftarrow> create_stack_frame (params@locals) values;
-    Some (sf#\<sigma>, \<gamma>, \<mu>)
+    sf \<leftarrow> create_locals_stack_frame (params@locals) values;
+    Some ((sf, Vr x)#\<sigma>, \<gamma>, \<mu>)
   }"
 
 (* Return eliminates the returning function's stack_frame, then assigns the result to the variable 
-   I did this because I wouldn't want to assign the result to a local variable in the stack_frame
-   that's going to be eliminated *)
-definition tr_return :: "vname \<Rightarrow> exp \<Rightarrow> transformer" where
-  "tr_return x a s = do {
+   or address where it's supposed to be assigned *)
+definition tr_return :: "exp \<Rightarrow> transformer" where
+  "tr_return a s = do {
     (v,(\<sigma>, \<gamma>, \<mu>)) \<leftarrow> eval a s;
-    s \<leftarrow> write_var x v (tl \<sigma>, \<gamma>, \<mu>);
-    Some s
-  }"
-
-(* Return eliminates the returning function's stack_frame *)
-definition tr_returnl :: "addr \<Rightarrow> exp \<Rightarrow> transformer" where
-  "tr_returnl addr a s = do {
-    (v,(\<sigma>, \<gamma>, \<mu>)) \<leftarrow> eval a s;
-    \<mu> \<leftarrow> store addr \<mu> v;
-    Some (tl \<sigma>, \<gamma>, \<mu>)
+    let ret = snd (hd \<sigma>);
+    case ret of
+      Vr x \<Rightarrow> do {
+        s \<leftarrow> write_var x v (tl \<sigma>, \<gamma>, \<mu>);
+        Some s
+      } |
+      Ar addr \<Rightarrow> do {
+        \<mu> \<leftarrow> store addr \<mu> v;
+        Some (tl \<sigma>, \<gamma>, \<mu>)
+      }
   }"
 
 
@@ -165,25 +164,20 @@ inductive cfg :: "com \<Rightarrow> cfg_label \<Rightarrow> com \<Rightarrow> bo
 | Assignl: "cfg (x ::== a) (en_always,tr_assignl x a) SKIP"
 | Seq1: "cfg (SKIP;; c\<^sub>2) (en_always, tr_id) c\<^sub>2"
 | Seq2: "\<lbrakk>cfg c\<^sub>1 a c\<^sub>1'\<rbrakk> \<Longrightarrow> cfg (c\<^sub>1;; c\<^sub>2) a (c\<^sub>1';; c\<^sub>2)"
-| Seq3: "cfg (Return a;; c\<^sub>2) (en_always, tr_id) (Return a)"
 | IfTrue: "cfg (IF b THEN c\<^sub>1 ELSE c\<^sub>2) (en_pos b, tr_eval b) c\<^sub>1"
 | IfFalse: "cfg (IF b THEN c\<^sub>1 ELSE c\<^sub>2) (en_neg b, tr_eval b) c\<^sub>2"
 | While: "cfg (WHILE b DO c) (en_always, tr_id) (IF b THEN c;; WHILE b DO c ELSE SKIP)"
 | Free: "cfg (FREE x) (en_always, tr_free x) SKIP"
 
-(* When we reach a return in a block we substitute by an assignment *)
-| Block1: "cfg (Block x (Return a)) (en_always, tr_return x a) SKIP"
-| Block2: "\<lbrakk>cfg c a c'\<rbrakk> \<Longrightarrow> cfg (Block x c) a (Block x c')"
-| Blockl1: "cfg (Blockl add (Return a)) (en_always, tr_returnl x a) SKIP"
-| Blockl2: "\<lbrakk>cfg c a c'\<rbrakk> \<Longrightarrow> cfg (Blockl x c) a (Blockl x c')"
+| Return: "cfg (Return a) (en_always, tr_return a) SKIP"
 
-(* Syntax for Callfun and Callfunl not working I think... *)
-| Callfun:
-    "cfg (Callfun x f params) (en_callfun f params, tr_callfun x f params)
-      (Block x (snd (snd (the (proc_table f)))))"
-(* I still have the problem with how to figure the address in which it will be saved.
-| Callfunl: "cfg (Callfunl x f params) pt (en_callfun f pt params, tr_callfunl pt x f params) (Block x (snd (snd (the (pt f)))))"
-*)
+| Block1: "\<lbrakk>cfg c\<^sub>1 (en, tr) c\<^sub>2; \<And>a. tr \<noteq> tr_return a\<rbrakk> \<Longrightarrow> cfg (Block c\<^sub>1) (en, tr) (Block c\<^sub>2)"
+| Block2: "cfg (Return a) (en, tr_return a) c\<^sub>2 \<Longrightarrow> cfg (Block (Return a)) (en, tr_id) SKIP"
+
+| Callfun: "cfg (Callfun x f params) (en_callfun f params, tr_callfun x f params)
+            (Block (snd (snd (the (proc_table f)))))"
+| Callfunl: "cfg (Callfunl x f params) (en_callfun f params, tr_callfunl x f params)
+            (Block (snd (snd (the (proc_table f)))))"
 
 (* A configuration can take a small step if there's a cfg edge between the two commands, the
    enabled returns True and the transformer successfully transforms the state into a new one.
@@ -219,8 +213,6 @@ apply (metis Assign Base not_None_eq small_step.intros(2))
   *)
 
 
-(* This doesn't hold anymore because the Return command can only happen in a Block but
-   there's no small step step from return to something else. *)
 lemma aux:
   assumes "c\<noteq>SKIP"
   shows "\<exists>x. (c,s) \<rightarrow> x"
@@ -272,16 +264,6 @@ next
         by (auto intro: small_step.None)
     qed
   qed
-      
-
-(*  {
-    assume "c\<^sub>1 = SKIP"
-    have ?case sorry
-  } moreover {
-    assume "c\<^sub>1 \<noteq> SKIP"
-    have ?case sorry
-  } ultimately show ?case by blast
-*)
 next
   case (If b c\<^sub>1 c\<^sub>2)
   show ?case
@@ -332,10 +314,22 @@ case (Free x)
       thus ?thesis using Free by auto
   qed
 next
+  case (Return a)
+    thus ?case
+    proof (cases "tr_return a s")
+      case None
+        hence "(Return a, s) \<rightarrow> None" using cfg.Return small_step.None by blast
+        thus ?thesis by auto
+    next
+      case (Some s\<^sub>2)
+        hence "(Return a, s) \<rightarrow> Some (SKIP, s\<^sub>2)" using cfg.Return small_step.Base by blast
+        thus ?thesis by auto
+    qed
+next
   case (Callfun x f params)
-  show ?case
+    thus ?case
     proof (cases "en_callfun f params s")
-      case (None)
+      case None
         hence "(Callfun x f params, s) \<rightarrow> None" using cfg.Callfun small_step.None by blast
         thus ?thesis by auto
     next
@@ -350,18 +344,49 @@ next
                 thus ?thesis by auto
             next
               case (Some s\<^sub>2)
-                hence "(Callfun x f params, s) \<rightarrow> Some (Block x (snd (snd (the (proc_table f)))), s\<^sub>2)" 
+                hence "(Callfun x f params, s) \<rightarrow> Some (Block (snd (snd (the (proc_table f)))), s\<^sub>2)" 
                   using True cfg.Callfun small_step.Base `en_callfun f params s = Some b` by metis
                 thus ?thesis by auto
             qed
         next
           case False
-          (* This case should never happen, I don't know how to prove this *)
-          thus ?thesis sorry
+            thus ?thesis (* This case should never happen, I don't know how to prove this *)
+            sorry
         qed
     qed
-qed 
-oops
+next
+  case (Callfunl x f params)
+    thus ?case
+    proof (cases "en_callfun f params s")
+      case None
+        hence "(Callfunl x f params, s) \<rightarrow> None" using cfg.Callfunl small_step.None by blast
+        thus ?thesis by auto
+    next
+      case (Some b)
+        show ?thesis
+        proof (cases b)
+          case True
+          show ?thesis
+            proof (cases "tr_callfunl x f params s")
+              case None
+                hence "(Callfunl x f params, s) \<rightarrow> None" using cfg.Callfunl small_step.None by blast
+                thus ?thesis by auto
+            next
+              case (Some s\<^sub>2)
+                hence "(Callfunl x f params, s) \<rightarrow> Some (Block (snd (snd (the (proc_table f)))), s\<^sub>2)" 
+                  using True cfg.Callfunl small_step.Base `en_callfun f params s = Some b` by metis
+                thus ?thesis by auto
+            qed
+        next
+          case False
+            thus ?thesis (* This case should never happen, I don't know how to prove this *)
+            sorry
+        qed
+    qed
+next
+  case (Block c)
+    thus ?case sorry
+qed
 
 
 lemma cfg_SKIP_stuck[simp]: "\<not> cfg SKIP a c"
@@ -397,17 +422,16 @@ lemma cfg_determ:
   apply (erule cfg.cases, auto) []
   apply (erule cfg.cases, auto) []
   apply (erule cfg.cases, auto) []
-  apply (erule cfg.cases, auto) []
   apply (rotate_tac)
   apply (erule cfg.cases, auto) []
   apply (erule cfg.cases, auto) []
-  prefer 2
-  apply (rotate_tac)
   apply (erule cfg.cases, auto) []
   apply (erule cfg.cases, auto) []
-  prefer 2
   apply (erule cfg.cases, auto) []
-  sorry
+  apply (erule cfg.cases, auto) []
+  apply (erule cfg.cases, auto) []
+  apply (erule cfg.cases, auto) []
+  done
 
 lemma small_step_determ:
   assumes "(c,s) \<rightarrow> c'"
@@ -438,7 +462,6 @@ fun fstep :: "com \<times> state \<Rightarrow> (com \<times> state) option" wher
     Some (SKIP,s)
   }"
 | "fstep (SKIP;;c, s) = Some (c,s)"
-| "fstep (Return a;; c, s) = Some (Return a, s)"
 | "fstep (c\<^sub>1;; c\<^sub>2, s) = do {
     (c\<^sub>1', s) \<leftarrow> fstep (c\<^sub>1, s);
     Some (c\<^sub>1' ;; c\<^sub>2, s)
@@ -453,32 +476,35 @@ fun fstep :: "com \<times> state \<Rightarrow> (com \<times> state) option" wher
     s \<leftarrow> tr_free x s;
     Some (SKIP, s)
   }"
+| "fstep (Return a, s) = do {
+    s \<leftarrow> tr_return a s;
+     Some (SKIP, s)
+  }"
+| "fstep (Block (Return a), s) = do {
+    (c, s) \<leftarrow> fstep (Return a, s);
+    Some (c, s)
+  }"
+| "fstep (Block c, s) = do {
+    (c, s) \<leftarrow> fstep (c, s);
+    Some (Block c, s)
+  }"
 | "fstep (Callfun x f params, s) = do {
     b \<leftarrow> en_callfun f params s;
     if b then do {
       s \<leftarrow> tr_callfun x f params s;
-      Some (Block x (snd (snd (the (proc_table f)))), s)
+      Some (Block (snd (snd (the (proc_table f)))), s)
     } else None
-}"
-| "fstep (Block x (Return a), s) = do {
-    s \<leftarrow> tr_return x a s;
-    Some (SKIP, s)
-}"
-| "fstep (Block x c, s) = do {
-    (c, s) \<leftarrow> fstep (c, s);
-    Some (Block x c, s)
-}"
-| "fstep (Blockl x (Return a), s) = do {
-    s \<leftarrow> tr_returnl x a s;
-    Some (SKIP, s)
-}"
-| "fstep (Blockl x c, s) = do {
-    (c, s) \<leftarrow> fstep (c, s);
-    Some (Blockl x c, s)
-}"
+  }"
+| "fstep (Callfunl x f params, s) = do {
+    b \<leftarrow> en_callfun f params s;
+    if b then do {
+      s \<leftarrow> tr_callfunl x f params s;
+      Some (Block (snd (snd (the (proc_table f)))), s)
+    } else None
+  }"
 
 
-lemma fstep_seq_nSKIP[simp]: "\<lbrakk>c\<^sub>1 \<noteq> SKIP; \<And>a. c\<^sub>1 \<noteq> Return a\<rbrakk> \<Longrightarrow> fstep (c\<^sub>1;; c\<^sub>2, s) = do {
+lemma fstep_seq_nSKIP[simp]: "c\<^sub>1 \<noteq> SKIP \<Longrightarrow> fstep (c\<^sub>1;; c\<^sub>2, s) = do {
     (c\<^sub>1', s) \<leftarrow> fstep (c\<^sub>1, s);
     Some (c\<^sub>1' ;; c\<^sub>2, s)
   }"
@@ -533,11 +559,6 @@ next
         using Base
         by simp
     next
-      case (Seq3 a)
-      thus ?thesis
-        using Base
-        by simp
-    next
       case (Seq2 cc\<^sub>1)
       hence [simp]: "c\<^sub>1 \<noteq> SKIP" by auto
 
@@ -545,8 +566,8 @@ next
         by (blast intro: small_step.intros)
       from Seq.IH(1)[OF this] have [simp]: "fstep (c\<^sub>1, s) = Some (cc\<^sub>1, s\<^sub>2)" by simp
 
-      show ?thesis using \<open>c\<^sub>1' = cc\<^sub>1;; c\<^sub>2\<close> sorry
-        (*by simp*)
+      show ?thesis using \<open>c\<^sub>1' = cc\<^sub>1;; c\<^sub>2\<close>
+        by simp
     qed
   next
     case (None en tr c\<^sub>1')
@@ -555,16 +576,14 @@ next
     proof cases
       case Seq1 with None(3) have False by auto thus ?thesis ..
     next
-      case Seq3 with None have False by auto thus ?thesis ..
-    next
       case (Seq2 cc1)
       hence [simp]: "c\<^sub>1 \<noteq> SKIP" by auto
 
       from None(3) Seq2(2) have "(c\<^sub>1,s) \<rightarrow> None"
         by (blast intro: small_step.intros)
       from Seq.IH(1)[OF this] have [simp]: "fstep (c\<^sub>1, s) = None" .
-      show ?thesis sorry
-        (*by simp*)
+      show ?thesis
+        by simp
     qed
   qed
 next
@@ -626,6 +645,20 @@ next
     qed
 print_cases
 next
+  case (Return a)
+    thus ?case
+    proof (cases "tr_return a s")
+      case None
+        hence "fstep (Return a, s) = None" by auto
+        moreover have "(Return a, s) \<rightarrow> None" using None cfg.Return small_step.None by blast
+        ultimately show ?thesis using Return small_step_determ by simp
+    next
+      case (Some s\<^sub>2)
+        hence "fstep (Return a, s) = Some (SKIP, s\<^sub>2)" by auto
+        moreover have "(Return a, s) \<rightarrow> Some (SKIP, s\<^sub>2)" using Some cfg.Return small_step.Base by blast
+        ultimately show ?thesis using Return small_step_determ by simp
+    qed
+next
   case (Callfun x f params)
     thus ?case
     proof (cases "en_callfun f params s")
@@ -647,9 +680,9 @@ next
                 ultimately show ?thesis using Callfun small_step_determ by simp
             next
               case (Some s\<^sub>2)
-                hence "fstep (Callfun x f params, s) = Some (Block x (snd (snd (the (proc_table f)))), s\<^sub>2)"
+                hence "fstep (Callfun x f params, s) = Some (Block (snd (snd (the (proc_table f)))), s\<^sub>2)"
                   using `en_callfun f params s = Some b` True by auto
-                moreover have "(Callfun x f params, s) \<rightarrow> Some (Block x (snd (snd (the (proc_table f)))), s\<^sub>2)" 
+                moreover have "(Callfun x f params, s) \<rightarrow> Some (Block (snd (snd (the (proc_table f)))), s\<^sub>2)" 
                   using True cfg.Callfun small_step.Base Some `en_callfun f params s = Some b` by metis
                 ultimately show ?thesis using Callfun small_step_determ by simp
             qed
@@ -660,13 +693,42 @@ next
         qed
     qed
 next
-  case (Return a) thus ?case sorry
+  case (Callfunl x f params)
+    thus ?case
+    proof (cases "en_callfun f params s")
+      case None
+        hence "fstep (Callfunl x f params, s) = None" by auto
+        moreover have "(Callfunl x f params, s) \<rightarrow> None" using None cfg.Callfunl small_step.None by blast
+        ultimately show ?thesis using Callfunl small_step_determ by simp
+    next
+      case (Some b)
+        thus ?thesis
+        proof (cases b)
+          case True
+            thus ?thesis
+            proof (cases "tr_callfunl x f params s")
+              case None
+                hence "fstep (Callfunl x f params, s) = None" using Some by auto
+                moreover have "(Callfunl x f params, s) \<rightarrow> None"
+                  using cfg.Callfunl small_step.None None by blast
+                ultimately show ?thesis using Callfunl small_step_determ by simp
+            next
+              case (Some s\<^sub>2)
+                hence "fstep (Callfunl x f params, s) = Some (Block (snd (snd (the (proc_table f)))), s\<^sub>2)"
+                  using `en_callfun f params s = Some b` True by auto
+                moreover have "(Callfunl x f params, s) \<rightarrow> Some (Block (snd (snd (the (proc_table f)))), s\<^sub>2)" 
+                  using True cfg.Callfunl small_step.Base Some `en_callfun f params s = Some b` by metis
+                ultimately show ?thesis using Callfunl small_step_determ by simp
+            qed
+        next
+          case False
+          (*This would never happen*)
+            thus ?thesis sorry
+        qed
+    qed
 next
-  case (Block x c) thus ?case sorry
-next
-  case (Blockl x c) thus ?case sorry
-next
-  case (Callfunl x f params) thus ?case sorry
+  case (Block c)
+    thus ?case sorry
 qed
 
 
@@ -788,6 +850,20 @@ next
         ultimately show ?thesis by auto
     qed
 next
+  case (Return a)
+    thus ?case
+    proof (cases "tr_return a s")
+      case None
+        hence "fstep (Return a, s) = None" by auto
+        moreover have "(Return a, s) \<rightarrow> None" using None cfg.Return small_step.None by blast
+        ultimately show ?thesis using Return small_step_determ by simp
+    next
+      case (Some s\<^sub>2)
+        hence "fstep (Return a, s) = Some (SKIP, s\<^sub>2)" by auto
+        moreover have "(Return a, s) \<rightarrow> Some (SKIP, s\<^sub>2)" using Some cfg.Return small_step.Base by blast
+        ultimately show ?thesis using Return small_step_determ by simp
+    qed
+next
   case (Callfun x f params)
     thus ?case
     proof (cases "en_callfun f params s")
@@ -809,9 +885,9 @@ next
                 ultimately show ?thesis using Callfun small_step_determ by simp
             next
               case (Some s\<^sub>2)
-                hence "fstep (Callfun x f params, s) = Some (Block x (snd (snd (the (proc_table f)))), s\<^sub>2)"
+                hence "fstep (Callfun x f params, s) = Some (Block (snd (snd (the (proc_table f)))), s\<^sub>2)"
                   using `en_callfun f params s = Some b` True by auto
-                moreover have "(Callfun x f params, s) \<rightarrow> Some (Block x (snd (snd (the (proc_table f)))), s\<^sub>2)" 
+                moreover have "(Callfun x f params, s) \<rightarrow> Some (Block (snd (snd (the (proc_table f)))), s\<^sub>2)" 
                   using True cfg.Callfun small_step.Base Some `en_callfun f params s = Some b` by metis
                 ultimately show ?thesis using Callfun small_step_determ by simp
             qed
@@ -822,13 +898,42 @@ next
         qed
     qed
 next
-  case (Return a) thus ?case sorry
+  case (Callfunl x f params)
+    thus ?case
+    proof (cases "en_callfun f params s")
+      case None
+        hence "fstep (Callfunl x f params, s) = None" by auto
+        moreover have "(Callfunl x f params, s) \<rightarrow> None" using None cfg.Callfunl small_step.None by blast
+        ultimately show ?thesis using Callfunl small_step_determ by simp
+    next
+      case (Some b)
+        thus ?thesis
+        proof (cases b)
+          case True
+            thus ?thesis
+            proof (cases "tr_callfunl x f params s")
+              case None
+                hence "fstep (Callfunl x f params, s) = None" using Some by auto
+                moreover have "(Callfunl x f params, s) \<rightarrow> None"
+                  using cfg.Callfunl small_step.None None by blast
+                ultimately show ?thesis using Callfunl small_step_determ by simp
+            next
+              case (Some s\<^sub>2)
+                hence "fstep (Callfunl x f params, s) = Some (Block (snd (snd (the (proc_table f)))), s\<^sub>2)"
+                  using `en_callfun f params s = Some b` True by auto
+                moreover have "(Callfunl x f params, s) \<rightarrow> Some (Block (snd (snd (the (proc_table f)))), s\<^sub>2)" 
+                  using True cfg.Callfunl small_step.Base Some `en_callfun f params s = Some b` by metis
+                ultimately show ?thesis using Callfunl small_step_determ by simp
+            qed
+        next
+          case False
+          (*This would never happen*)
+            thus ?thesis sorry
+        qed
+    qed
 next
-  case (Block x c) thus ?case sorry
-next
-  case (Blockl x c) thus ?case sorry
-next
-  case (Callfunl x f params) thus ?case sorry
+  case (Block c)
+    thus ?case sorry
 qed
 
 
